Proving examples/bytes/Platform.Bytes.fst

examples/bytes/Platform.Bytes.fst
@@ -1,228 +1,277 @@
 module Platform.Bytes
 open FStar
 open FStar.List
+open FStar.List.Tot
 
-  val repr_bytes : nat -> GTot (n:nat{n>0})
-  let repr_bytes n =
-      if n < 256 then 1
-      else if n < 65536 then 2
-      else if n < 16777216 then 3
-      else if n < 4294967296 then 4
-      else if n < 1099511627776 then 5
-      else if n < 281474976710656 then 6
-      else if n < 72057594037927936 then 7
-      else if n < 18446744073709551616 then 8
-      else 9
+val repr_bytes : nat -> GTot (n:nat{n>0})
+let repr_bytes n =
+    if n < 256 then 1
+    else if n < 65536 then 2
+    else if n < 16777216 then 3
+    else if n < 4294967296 then 4
+    else if n < 1099511627776 then 5
+    else if n < 281474976710656 then 6
+    else if n < 72057594037927936 then 7
+    else if n < 18446744073709551616 then 8
+    else 9
 
-  val lemma_repr_bytes_values: n:nat ->
-    Lemma (   ( n < 256 <==> repr_bytes n = 1 )
-           /\ ( (n >= 256 /\ n < 65536) <==> repr_bytes n = 2 )
-           /\ ( (n >= 65536 /\ n < 16777216) <==> repr_bytes n = 3 )
-           /\ ( (n >= 16777216 /\ n < 4294967296) <==> repr_bytes n = 4 )
-           /\ ( (n >= 4294967296 /\ n < 1099511627776) <==> repr_bytes n = 5 )
-           /\ ( (n >= 1099511627776 /\ n < 281474976710656) <==> repr_bytes n = 6 )
-           /\ ( (n >= 281474976710656 /\ n < 72057594037927936) <==> repr_bytes n = 7 )
-           /\ ( (n >= 72057594037927936 /\ n < 18446744073709551616) <==> repr_bytes n = 8 ) )
-  let lemma_repr_bytes_values n = ()
+val lemma_repr_bytes_values: n:nat ->
+  Lemma (   ( n < 256 <==> repr_bytes n = 1 )
+         /\ ( (n >= 256 /\ n < 65536) <==> repr_bytes n = 2 )
+         /\ ( (n >= 65536 /\ n < 16777216) <==> repr_bytes n = 3 )
+         /\ ( (n >= 16777216 /\ n < 4294967296) <==> repr_bytes n = 4 )
+         /\ ( (n >= 4294967296 /\ n < 1099511627776) <==> repr_bytes n = 5 )
+         /\ ( (n >= 1099511627776 /\ n < 281474976710656) <==> repr_bytes n = 6 )
+         /\ ( (n >= 281474976710656 /\ n < 72057594037927936) <==> repr_bytes n = 7 )
+         /\ ( (n >= 72057594037927936 /\ n < 18446744073709551616) <==> repr_bytes n = 8 ) )
+let lemma_repr_bytes_values n = ()
 
-  type byte = Char.char
+type byte = Char.char
+type cbytes = string
 
-  type cbytes = string
+(* let add_nat (a : nat) (b : nat) : nat = a + b *)
 
-  (* let add_nat (a : nat) (b : nat) : nat = a + b *)
+(* val sum : list nat -> Tot nat *)
+(* let sum ls = fold_leftT add_nat 0 ls *)
 
-  (* val sum : list nat -> Tot nat *)
-  (* let sum ls = fold_leftT add_nat 0 ls *)
+val sum_length : list string -> Tot nat
+(* let sum_length ls = sum (mapT String.length ls) *)
+let rec sum_length ls =
+  match ls with
+  | [] -> 0
+  | h :: t -> String.length h + sum_length t
 
-  val sum_length : list string -> Tot nat
-  (* let sum_length ls = sum (mapT String.length ls) *)
-  let rec sum_length ls =
-    match ls with
-    | [] -> 0
-    | h :: t -> String.length h + sum_length t
+type proto_bytes = {
+       (*  A series of strings whose total concatenated length is [max]. *)
+       bl: list cbytes;
+       max: nat;
+       (* The length of the subset. *)
+       length: nat;
+       (* The start index of the subset. *)
+       index: nat
+}
 
-  type proto_bytes = {
-         (*  A series of strings whose total concatenated length is [max]. *)
-         bl: list cbytes;
-         max: nat;
-         (* The length of the subset. *)
-         length: nat;
-         (* The start index of the subset. *)
-         index: nat
-  }
+type good_bytes (b:proto_bytes) = b.max = sum_length b.bl /\ b.index <= b.max /\ b.index + b.length <= b.max
 
-  type good_bytes (b:proto_bytes) = b.max = sum_length b.bl /\ b.index <= b.max /\ b.index + b.length <= b.max
+type bytes = b:proto_bytes{good_bytes b}
 
-  type bytes = b:proto_bytes{good_bytes b}
+(* type bytes =  *)
+(*   | MkBytes :  *)
+(*        (\*  A series of strings whose total concatenated length is [max]. *\) *)
+(*        bl: list cbytes -> *)
+(*        max: nat -> *)
+(*        (\* The length of the subset. *\) *)
+(*        length: nat -> *)
+(*        (\* The start index of the subset. *\) *)
+(*        index: nat{max = sum_length bl /\ index <= max /\ index + length <= max} -> *)
+(*        bytes *)
 
-  (* type bytes =  *)
-  (*   | MkBytes :  *)
-  (*        (\*  A series of strings whose total concatenated length is [max]. *\) *)
-  (*        bl: list cbytes -> *)
-  (*        max: nat -> *)
-  (*        (\* The length of the subset. *\) *)
-  (*        length: nat -> *)
-  (*        (\* The start index of the subset. *\) *)
-  (*        index: nat{max = sum_length bl /\ index <= max /\ index + length <= max} -> *)
-  (*        bytes *)
+assume val substringT: s:string -> start:nat -> len:nat{let l = String.length s in start <= l && start + len <= l} -> Tot (res:string{String.length res = len})
+assume val string_length_append: a:string -> b:string -> Lemma (String.length (a ^ b) = String.length a + String.length b)
+assume val string_length_empty: unit -> Lemma (String.length "" = 0)
 
-  let rec getByte (bl:list cbytes) (i:int) =
+val string_append : a:string -> b:string -> Tot (res:string{String.length res = String.length a + String.length b})
+let string_append a b = 
+  let _ = string_length_append a b in 
+  a ^ b
+val empty_string : s:string{String.length s = 0}
+let empty_string = 
+  let _ = string_length_empty () in
+  ""
+
+(* val sum_length_le : i:nat -> h:cbytes -> t:list cbytes -> Lemma (i <= sum_length (h::t) ==> i - String.length h <= sum_length t) *)
+(* let sum_length_le i h t = () *)
+
+(* val sum_length_cons : h:cbytes -> t:list cbytes -> Lemma (sum_length (h::t) = String.length h + sum_length t) (decreases t) *)
+(* let rec sum_length_cons h t =  *)
+(*   match t with *)
+(*    | [] -> () *)
+(*    | h' :: t' -> sum_length_cons h' t' *)
+
+val exfalso : #a:Type -> u:unit{False} -> Tot a
+let rec exfalso #a _ = exfalso ()
+
+val getBytes : bl:list cbytes -> i:nat{i <= sum_length bl} -> n:nat{i+n <= sum_length bl} -> Tot (b:cbytes{String.length b = n})
+let rec getBytes (bl: list cbytes) i n  =
     match bl with
-      | [] -> failwith "getByte: array out of bounds"
-      | h::t -> 
-        if i >= String.length h then 
-          getByte t (i-String.length h)
-        else 
-          String.get h i
+    | [] -> 
+      if n = 0
+      then empty_string
+      else exfalso ()
+    | h::t ->
+        if i >= (String.length h)
+        then getBytes t (i- (String.length h)) n
+        else let curr = (String.length h) - i in
+             if curr >= n
+             then substringT h i n
+             else 
+             string_append (substringT h i curr) (getBytes t 0 (n-curr))
 
-  let rec getByte2 (bl: list cbytes) i : byte * byte =
-      match bl with
-     | [] -> failwith "array out of bounds"
-     | h::t -> 
-       if i >= String.length h then 
-         getByte2 t (i - String.length h)
-       else if (String.length h) - i >= 2 then 
-         (String.get h i, String.get h (i+1))
-       else 
-       match bl with
-       | h1::h2::t ->
-         if (String.length h1) - i = 1 && (String.length h2) > 0 then 
-           (String.get h1 i, String.get h2 0)
-         else failwith "getByte2: array out of bounds"
-       | _ -> failwith "getByte2: array out of bounds"
+val string_concat : ls:list string -> Tot (r:string{String.length r = sum_length ls})
+let rec string_concat ls =
+  match ls with
+  | [] -> empty_string
+  | x :: xs -> string_append x (string_concat xs)
 
-  assume val substringT: s:string -> start:nat -> len:nat{let l = String.length s in start <= l && start + len <= l} -> Tot (res:string{String.length res = len})
-  assume val string_length_concat: a:string -> b:string -> Lemma (String.length (a ^ b) = String.length a + String.length b)
-  assume val string_length_empty: unit -> Lemma (String.length "" = 0)
-
-  val string_concat : a:string -> b:string -> Tot (res:string{String.length res = String.length a + String.length b})
-  let string_concat a b = 
-    let _ = string_length_concat a b in 
-    a ^ b
-  val empty_string : s:string{String.length s = 0}
-  let empty_string = 
-    let _ = string_length_empty () in
-    ""
-
-  (* val sum_length_le : i:nat -> h:cbytes -> t:list cbytes -> Lemma (i <= sum_length (h::t) ==> i - String.length h <= sum_length t) *)
-  (* let sum_length_le i h t = () *)
-
-  (* val sum_length_cons : h:cbytes -> t:list cbytes -> Lemma (sum_length (h::t) = String.length h + sum_length t) (decreases t) *)
-  (* let rec sum_length_cons h t =  *)
-  (*   match t with *)
-  (*    | [] -> () *)
-  (*    | h' :: t' -> sum_length_cons h' t' *)
-
-  val getBytes : bl:list cbytes -> i:nat{i <= sum_length bl} -> n:nat{i+n <= sum_length bl} -> Tot (b:cbytes{String.length b = n})
-  let rec getBytes (bl: list cbytes) i n  =
-      match bl with
-      | [] -> 
-        if n = 0
-        then empty_string
-        else admit() (*ToDo: should be 'exfalso'*)
-      | h::t ->
-          if i >= (String.length h)
-          then getBytes t (i- (String.length h)) n
-          else let curr = (String.length h) - i in
-               if curr >= n
-               then substringT h i n
-               else 
-               string_concat (substringT h i curr) (getBytes t 0 (n-curr))
-
-  let cbyte (b:bytes) =
-    if b.length = 1 then
-      let b1 = getByte b.bl b.index in b1
-    else failwith "cbyte: expected an array of length 1"
-
-  let cbyte2 (b:bytes) =
-      if b.length = 2 then
-        let (b1,b2) = getByte2 b.bl b.index in b1,b2
-      else failwith "cbyte2: expected an array of length 2"
-
-  let index (b:bytes) i =
-    if b.length >= i then
-      let s = getBytes b.bl b.index b.length in
-      String.get s i
-    else failwith "index: index out of range"
-
-  val string_concat_all : ls:list string -> Tot (r:string{String.length r = sum_length ls})
-  let rec string_concat_all ls =
-    match ls with
-    | [] -> empty_string
-    | x :: xs -> string_concat x (string_concat_all xs)
-  
-  val get_cbytes : b:bytes -> Tot (r:cbytes{String.length r = b.length})
-  let get_cbytes (b:bytes) =
-      if b.length = b.max && b.index = 0 then
-        string_concat empty_string (string_concat_all b.bl)
-      else
-        getBytes b.bl b.index b.length
-
-  let abytes (ba:cbytes) =
-      {bl = [ba]; length = String.length ba; index = 0; max = String.length ba}
-
-  (* let rec for_ first last init f = *)
-  (*   if first > last then *)
-  (*     init *)
-  (*   else *)
-  (*     for_ (first + 1) last (f init first) f *)
-
-  let abytes_max (ba:cbytes) (max:int) =
-    let len = String.length ba in
-    if len <= max then
-      let arr = ba ^ String.make (max-len) (Char.char_of_int 0) in
-      {bl = [arr]; length = len; index = 0; max = len}
+val get_cbytes : b:bytes -> Tot (r:cbytes{String.length r = b.length})
+let get_cbytes (b:bytes) =
+    if b.length = b.max && b.index = 0 then
+      string_concat b.bl
     else
-      failwith "abytes_max: length exceeds max"
+      getBytes b.bl b.index b.length
 
-  let abyte (ba:byte) =
-      {bl = [String.make 1 ba]; length = 1; index = 0; max = 1}
+val sum_length_append : a:list string -> b:list string -> Lemma (sum_length (a @ b) = sum_length a + sum_length b)
+let rec sum_length_append a b =
+  match a with
+    | [] -> ()
+    | x :: a' -> sum_length_append a' b
 
-  let abyte2 (ba1,ba2) =
-      let s = String.make 1 ba1 ^ String.make 1 ba2 in
-      {bl = [s]; length = 2; index = 0; max = 2}
+val op_At_Bar: bytes -> bytes -> Tot bytes
+let op_At_Bar (a:bytes) (b:bytes) =
+    if a.length + a.index = a.max && b.index = 0 then
+      let _ = sum_length_append a.bl b.bl in
+      {bl = (a.bl @ b.bl);
+       length = a.length + b.length;
+       index = a.index;
+       max = a.max + b.max}
+    else
+      {bl = [string_append (get_cbytes a) (get_cbytes b)];
+       length = a.length + b.length;
+       index = 0;
+       max = a.length + b.length}
 
-  val sum_length_concat : a:list string -> b:list string -> Lemma (sum_length (a @ b) = sum_length a + sum_length b)
-  let rec sum_length_concat a b =
-    match a with
-      | [] -> ()
-      | x :: a' -> sum_length_concat a' b
+let op_AtBar = op_At_Bar
 
-  val op_At_Bar: bytes -> bytes -> Tot bytes
-  let op_At_Bar (a:bytes) (b:bytes) =
-      if a.length + a.index = a.max && b.index = 0 then
-        let _ = sum_length_concat a.bl b.bl in
-        {bl = (a.bl @ b.bl);
-         length = a.length + b.length;
-         index = a.index;
-         max = a.max + b.max}
-      else
-        {bl = [string_concat (get_cbytes a) (get_cbytes b)];
-         length = a.length + b.length;
-         index = 0;
-         max = a.length + b.length}
+val lemma_op_At_Bar : a:bytes -> b:bytes -> Lemma (get_cbytes (a @| b) = (get_cbytes a ^ get_cbytes b))
 
-  let op_AtBar = op_At_Bar
+assume val append_empty : unit -> Lemma (forall s. s ^ "" = s)
+assume Append_empty : forall s. s ^ "" = s
+assume val empty_append : unit -> Lemma (forall s. ("" ^ s) = s)
+assume Empty_append: forall s. "" ^ s = s
+assume val append_assoc : unit -> Lemma (forall a b c. (a ^ (b ^ c)) = ((a ^ b) ^ c))
+assume Append_assoc : forall a b c. (a ^ (b ^ c)) = ((a ^ b) ^ c)
 
-  let length (d:bytes) = d.length
+val concat_append : a:list string -> b:list string -> Lemma (string_concat (a @ b) = (string_concat a ^ string_concat b))
+let rec concat_append a b =
+  match a with
+    | [] -> 
+    let _ = empty_append () in
+    ()
+    | x :: xs -> 
+    let _ = append_assoc () in
+    let _ = concat_append xs b in
+    ()
 
-  type bytes_eq (a:bytes) (b:bytes) = (get_cbytes a = get_cbytes b)
-  
-  val split : s:bytes -> i:nat{i <= length s} -> Tot (x:(bytes * bytes){length (fst x) = i && length (snd x) = length s - i /\ bytes_eq ((fst x) @| (snd x)) s})
-  let split (b:bytes) (i:nat{i <= length b}) =
-      {bl = b.bl;
-       length = i;
-       index = b.index;
-       max = b.max},
-      {bl = b.bl;
-       length = b.length - i;
-       index = b.index + i;
-       max = b.max}
+let lemma_op_At_Bar a b =
+  let c = a @| b in
+  if a.length + a.index = a.max && b.index = 0 then
+    if a.index = 0 then
+      ()
+    else
+      admit ()
+  else
+    if c.length = c.max && c.index = 0 then
+      let _ = append_empty (string_append (get_cbytes a) (get_cbytes b)) in
+      ()
+    else
+      exfalso ()
+    
+let abytes (ba:cbytes) =
+    {bl = [ba]; length = String.length ba; index = 0; max = String.length ba}
 
-  val split_eq: s:bytes -> i:nat{(0 <= i /\ i <= length s)} -> Pure
-    (x:(bytes * bytes){length (fst x) = i && length (snd x) = length s - i})
-    (requires True)
-    (ensures (fun x -> ((fst x) @| (snd x) = s)))
-  
-  let split_eq = split
+(* let rec for_ first last init f = *)
+(*   if first > last then *)
+(*     init *)
+(*   else *)
+(*     for_ (first + 1) last (f init first) f *)
+
+let abytes_max (ba:cbytes) (max:int) =
+  let len = String.length ba in
+  if len <= max then
+    let arr = ba ^ String.make (max-len) (Char.char_of_int 0) in
+    {bl = [arr]; length = len; index = 0; max = len}
+  else
+    failwith "abytes_max: length exceeds max"
+
+let abyte (ba:byte) =
+    {bl = [String.make 1 ba]; length = 1; index = 0; max = 1}
+
+let abyte2 (ba1,ba2) =
+    let s = String.make 1 ba1 ^ String.make 1 ba2 in
+    {bl = [s]; length = 2; index = 0; max = 2}
+
+let length (d:bytes) = d.length
+
+val getByte : list cbytes -> int -> Char.char
+let rec getByte (bl:list cbytes) (i:int) =
+  match bl with
+    | [] -> failwith "getByte: array out of bounds"
+    | h::t -> 
+      if i >= String.length h then 
+        getByte t (i-String.length h)
+      else 
+        String.get h i
+
+val getByte2 : list cbytes -> int -> byte * byte
+let rec getByte2 (bl: list cbytes) i =
+    match bl with
+   | [] -> failwith "array out of bounds"
+   | h::t -> 
+     if i >= String.length h then 
+       getByte2 t (i - String.length h)
+     else if (String.length h) - i >= 2 then 
+       (String.get h i, String.get h (i+1))
+     else 
+     match bl with
+     | h1::h2::t ->
+       if (String.length h1) - i = 1 && (String.length h2) > 0 then 
+         (String.get h1 i, String.get h2 0)
+       else failwith "getByte2: array out of bounds"
+     | _ -> failwith "getByte2: array out of bounds"
+
+let cbyte (b:bytes) =
+  if b.length = 1 then
+    let b1 = getByte b.bl b.index in b1
+  else failwith "cbyte: expected an array of length 1"
+
+let cbyte2 (b:bytes) =
+    if b.length = 2 then
+      let (b1,b2) = getByte2 b.bl b.index in b1,b2
+    else failwith "cbyte2: expected an array of length 2"
+
+assume val getT: s:string -> i:int{i < String.length s} -> Char.char
+
+let index (b:bytes) i =
+  if b.length > i then
+    let s = getBytes b.bl b.index b.length in
+    getT s i
+  else failwith "index: index out of range"
+
+type bytes_eq (a:bytes) (b:bytes) = (get_cbytes a = get_cbytes b)
+
+val split : s:bytes -> i:nat{i <= length s} -> Tot (bytes * bytes)
+let split b i =
+    {bl = b.bl;
+     length = i;
+     index = b.index;
+     max = b.max},
+    {bl = b.bl;
+     length = b.length - i;
+     index = b.index + i;
+     max = b.max}
+
+val lemma_split_1 : s:bytes -> i:nat{i <= length s} -> Lemma (let x = split s i in length (fst x) = i && length (snd x) = length s - i)
+let lemma_split_1 s i = ()
+
+val lemma_split2 : s:bytes -> i:nat{i <= length s} -> Lemma (let x = split s i in bytes_eq ((fst x) @| (snd x)) s)
+let lemma_split2 s i = ()
+
+val split_eq : s:bytes -> i:nat{i <= length s} -> Tot (x:(bytes * bytes){length (fst x) = i && length (snd x) = length s - i /\ bytes_eq ((fst x) @| (snd x)) s})
+let split_eq = 
+  split
+
+(* val split_eq: s:bytes -> i:nat{(0 <= i /\ i <= length s)} -> Pure *)
+(*   (x:(bytes * bytes){length (fst x) = i && length (snd x) = length s - i}) *)
+(*   (requires True) *)
+(*   (ensures (fun x -> ((fst x) @| (snd x) = s))) *)
 
